

FOURIER SERIES

- A function $f(x)$ is called a **periodic function** if $f(x)$ is defined for all real x , except possibly at some points, and if there is some positive number p , called a **period** of $f(x)$ such that

$$f(x + p) = f(x) \quad \text{for all } x$$

- Familiar periodic functions are the *cosine*, *sine*, *tangent*, and *cotangent*. Examples of functions that are not periodic are $x, x^2, x^3, e^x, \cos hx$ etc. to mention just a few.

If $f(x)$ has a period of p then it has also a period of $2p$

$$f(x + 2p) = f\{(x + p) + p\} = f(x + p) = f(x)$$

Or in general we can write

$$f(x + np) = f(x)$$

- A Fourier series is defined as an expansion of a real function or representation of a real function in a series of sines and cosines such as

$$f(x) = \frac{a_0}{2} + \sum_{n=1}^{\infty} a_n \cos nx + \sum_{n=1}^{\infty} b_n \sin nx$$

Where a_0, a_n , and b_n are constants, called the **Fourier coefficients** of the series. We see that each term has the period of 2π Hence *if the coefficients are such that the series converges, its sum will be a function of period 2π .*

- The **Fourier coefficients** of $f(x)$, given by the **Euler formulas**

$$a_0 = \frac{1}{2\pi} \int_{-\pi}^{\pi} f(x) dx$$

$$a_n = \frac{1}{\pi} \int_{-\pi}^{\pi} f(x) \cos nx \, dx \quad n = 1, 2, 3, \dots$$

$$b_n = \frac{1}{\pi} \int_{-\pi}^{\pi} f(x) \sin nx \, dx \quad n = 1, 2, 3, \dots$$

The above Fourier series is given for period 2π . The transition from period 2π to be period $p = 2L$ is effected by a suitable change of scale, as follows. Let $f(x)$ have period $= 2L$. Then we can introduce a new variable v such that $f(x)$ as a function of v , has period 2π .

- If we set

$$x = \frac{p}{2\pi} v \Rightarrow v = \frac{2\pi}{p} x \Rightarrow v = \frac{\pi}{L} x$$

This means $v = \pm\pi$ corresponds to $x = \pm L$. This represents f , as a function of v has a period of 2π . Hence the Fourier series is

$$f(v) = \frac{a_0}{2} + \sum_{n=1}^{\infty} a_n \cos nv + \sum_{n=1}^{\infty} b_n \sin nv$$

- Now using $v = \frac{\pi}{L} x$ Fourier series for the period of $(-L, L)$ is given by

$$f(x) = \frac{a_0}{2} + \sum_{n=1}^{\infty} a_n \cos n \frac{\pi}{L} x + \sum_{n=1}^{\infty} b_n \sin n \frac{\pi}{L} x$$

This is Fourier series we obtain for a function of $f(x)$ period $2L$ the Fourier series.

The coefficient is given by

$$a_0 = \frac{1}{L} \int_{-L}^L f(t) dt,$$

$$a_n = \frac{1}{L} \int_{-L}^L f(x) \cos \frac{n\pi x}{L} dx,$$

- $b_n = \frac{1}{L} \int_{-L}^L f(x) \sin \frac{n\pi x}{L} dx,$

SOME IMPORTANT RESULTS

- $\int e^{ax} \sin bx \, dx = \frac{e^{ax}}{a^2 + b^2} (a \sin bx - b \cos bx)$
- $\int e^{ax} \cos bx \, dx = \frac{e^{ax}}{a^2 + b^2} (a \cos bx + b \sin bx)$
- $\int_0^{\infty} \frac{\sin ax}{x} \, dx = \frac{\pi}{2}$
- $\int_0^{\infty} e^{-x^2} \, dx = \frac{\sqrt{\pi}}{2}$
- $\int_{-\infty}^{\infty} \frac{\sin mx}{(x-b)^2 + a^2} \, dx = \frac{\pi}{a} e^{-am} \sin bm, \quad [m > 0]$

FOURIER INTEGRAL

- Fourier series are powerful tools for problems involving functions that are periodic or are of interest on a finite interval only.
- Since, of course, many problems involve functions that are **nonperiodic and are of interest on the whole x -axis**, we ask what can be done to extend the method of Fourier series to such functions. This idea will lead to “Fourier integrals.”

FOURIER INTEGRAL THEOREM

Fourier integral theorem states that $f(x) = \frac{1}{\pi} \int_0^\infty \int_{-\infty}^\infty f(t) \cos u(t-x) dt du$

Proof. We know that Fourier series of a function $f(x)$ in $(-c, c)$ is given by

$$f(x) = \frac{a_0}{2} + \sum_{n=1}^\infty a_n \cos \frac{n\pi x}{c} + \sum_{n=1}^\infty b_n \sin \frac{n\pi x}{c}$$

Where a_0 , a_n and b_n are given by

$$\begin{aligned} a_0 &= \frac{1}{c} \int_{-c}^c f(t) dt, \\ a_n &= \frac{1}{c} \int_{-c}^c f(t) \cos \frac{n\pi t}{c} dt, \\ b_n &= \frac{1}{c} \int_{-c}^c f(t) \sin \frac{n\pi t}{c} dt, \end{aligned}$$

Substituting the values of a_0 , a_n and b_n in above equation, we get

$$f(x) = \frac{1}{2c} \int_{-c}^c f(t) dt + \sum_{n=1}^\infty \frac{1}{c} \int_{-c}^c f(t) \cos \frac{n\pi t}{c} dt \cos \frac{n\pi x}{c} + \sum_{n=1}^\infty \frac{1}{c} \int_{-c}^c f(t) \sin \frac{n\pi t}{c} dt \sin \frac{n\pi x}{c}$$

$$f(x) = \frac{1}{2c} \int_{-c}^c f(t) dt + \sum_{n=1}^\infty \frac{1}{c} \int_{-c}^c f(t) \left[\cos \frac{n\pi t}{c} \cos \frac{n\pi x}{c} + \sin \frac{n\pi t}{c} \sin \frac{n\pi x}{c} \right] dt$$

$$f(x) = \frac{1}{2c} \int_{-c}^c f(t) dt + \sum_{n=1}^\infty \frac{1}{c} \int_{-c}^c f(t) \left[\cos \left(\frac{n\pi t}{c} - \frac{n\pi x}{c} \right) \right] dt$$

$$f(x) = \frac{1}{2c} \int_{-c}^c f(t) dt + \sum_{n=1}^\infty \frac{1}{c} \int_{-c}^c f(t) \left[\cos \frac{n\pi}{c} (t-x) \right] dt$$

$$f(x) = \frac{1}{2c} \int_{-c}^c f(t) \left\{ 1 + 2 \sum_{n=1}^\infty \cos \frac{n\pi}{c} (t-x) \right\} dt$$

Since cosine functions are even functions i.e., $\cos(-\theta) = \cos \theta$ the expression

$$\left\{ 1 + 2 \sum_{n=1}^\infty \cos \frac{n\pi}{c} (t-x) \right\} = \sum_{n=-\infty}^\infty \cos \frac{n\pi}{c} (t-x)$$

We now let the parameter c approach infinity, transforming the finite interval $[-c, c]$ into the infinite interval $(-\infty$ to $+\infty)$. We set

$$\frac{n\pi}{c} = \omega, \text{ and } \frac{\pi}{c} = d\omega \quad \text{with } c \rightarrow \infty$$

Then we have

$$f(x) = \frac{1}{2\pi} \int_{-\infty}^\infty f(t) \left\{ \int_{-\infty}^\infty d\omega \cos \omega(t-x) \right\} dt$$

On simplifying

$$f(x) = \frac{1}{\pi} \int_0^\infty \int_{-\infty}^\infty f(t) \cos \omega(t-x) d\omega dt \quad \text{Proved}$$

FOURIER SINE AND COSINE INTEGRALS

$$f(x) = \frac{2}{\pi} \int_0^{\infty} \sin \omega x \, d\omega \int_0^{\infty} f(t) \sin \omega t \, dt \quad (\text{Fourier Sine Integrals})$$

$$f(x) = \frac{2}{\pi} \int_0^{\infty} \cos \omega x \, d\omega \int_0^{\infty} f(t) \cos \omega t \, dt \quad (\text{Fourier Cosine Integrals})$$

Proof: We can write

$$\cos \omega(t - x) = \cos(\omega t - \omega x) = \cos \omega t \cos \omega x + \sin \omega t \sin \omega x$$

Using this expansion in Fourier integral theorem, we have

$$\begin{aligned} f(x) &= \frac{1}{\pi} \int_0^{\infty} \int_{-\infty}^{\infty} \cos \omega(t - x) \, d\omega \, dt \\ \Rightarrow f(x) &= \frac{1}{\pi} \int_0^{\infty} \int_{-\infty}^{\infty} f(t) (\cos \omega t \cos \omega x + \sin \omega t \sin \omega x) \, d\omega \, dt \\ \Rightarrow f(x) &= \frac{1}{\pi} \int_0^{\infty} \int_{-\infty}^{\infty} f(t) (\cos \omega t \cos \omega x \, d\omega \, dt + \frac{1}{\pi} \int_0^{\infty} \int_{-\infty}^{\infty} f(t) \sin \omega t \sin \omega x \, d\omega \, dt \end{aligned}$$

Now to solve the above equation, we have two different cases, using the following conditions

$$\int_{-a}^a f(x) \, dx = 0 \quad \text{for odd function}$$

And

$$\int_{-a}^a f(x) \, dx = 2 \int_0^a f(x) \, dx \quad \text{for even function}$$

Case I: when $f(t)$ is even function: this means

$$\Rightarrow f(t) \sin \omega t \quad \text{is odd function and} \\ f(t) \cos \omega t \quad \text{is even function}$$

Hence

$$\frac{1}{\pi} \int_0^{\infty} \int_{-\infty}^{\infty} f(t) \sin \omega t \sin \omega x \, d\omega \, dt = 0$$

And

$$\Rightarrow f(x) = \frac{1}{\pi} \int_0^{\infty} \int_{-\infty}^{\infty} f(t) (\cos \omega t \cos \omega x \, d\omega \, dt = \frac{2}{\pi} \int_0^{\infty} \cos \omega x \, d\omega \int_{-\infty}^{\infty} f(t) \cos \omega t \, dt$$

$$f(x) = \frac{2}{\pi} \int_0^{\infty} \cos \omega x \, d\omega \int_0^{\infty} f(t) \cos \omega t \, dt$$

Case II: If $f(t)$ is odd function: this means

$$\Rightarrow f(t) \sin \omega t \quad \text{is even function and} \\ f(t) \cos \omega t \quad \text{is odd function}$$

Hence

$$\frac{1}{\pi} \int_0^{\infty} \int_{-\infty}^{\infty} f(t) \cos \omega t \cos \omega x \, d\omega \, dt = 0$$

And

$$\begin{aligned} \Rightarrow f(x) &= \frac{1}{\pi} \int_0^{\infty} \int_{-\infty}^{\infty} f(t) \sin \omega t \sin \omega x \, d\omega \, dt = \frac{2}{\pi} \int_0^{\infty} \sin \omega x \, d\omega \int_{-\infty}^{\infty} f(t) \sin \omega t \, dt \\ f(x) &= \frac{2}{\pi} \int_0^{\infty} \sin \omega x \, d\omega \int_0^{\infty} f(t) \sin \omega t \, dt \end{aligned}$$

This is known as Fourier sine integral.

FOURIER'S COMPLEX INTEGRALS

We know from Fourier integral theorem

$$f(x) = \frac{1}{2\pi} \int_{-\infty}^{\infty} \int_{-\infty}^{\infty} f(t) \cos \omega(t-x) d\omega dt$$

Now adding

$$f(x) = \frac{i}{2\pi} \int_{-\infty}^{\infty} f(t) dt \int_{-\infty}^{\infty} \sin \omega(t-x) d\omega = 0$$

Since

$$\int_{-\infty}^{\infty} \sin \omega(t-x) d\omega = 0 \quad \text{because of odd function}$$

Hence

$$f(x) = \frac{1}{2\pi} \int_{-\infty}^{\infty} \int_{-\infty}^{\infty} f(t) \cos \omega(t-x) d\omega dt + \frac{i}{2\pi} \int_{-\infty}^{\infty} f(t) dt \int_{-\infty}^{\infty} \sin \omega(t-x) d\omega$$

$$f(x) = \frac{1}{2\pi} \int_{-\infty}^{\infty} f(t) dt \left[\int_{-\infty}^{\infty} \cos \omega(t-x) + i \sin \omega(t-x) \right] d\omega$$

$$f(x) = \frac{1}{2\pi} \int_{-\infty}^{\infty} f(t) dt \left[\int_{-\infty}^{\infty} e^{i\omega(t-x)} \right] d\omega$$

$$f(x) = \frac{1}{2\pi} \int_{-\infty}^{\infty} e^{-i\omega x} d\omega \int_{-\infty}^{\infty} f(t) e^{i\omega t} dt$$

This relation is known as Fourier's complex Integral.

Example 1. Express the following function

$$f(x) = \begin{cases} 1 & \text{when } x \leq 1 \\ 0 & \text{when } x > 1 \end{cases}$$

as a Fourier integral. Hence evaluate

$$\int_0^{\infty} \frac{\sin u \cos ux}{u} du$$

Solution: we know the Fourier Integral theorem, the Fourier Integral of a function $f(x)$ is given by

$$f(x) = \frac{1}{\pi} \int_0^{\infty} \int_{-\infty}^{\infty} f(t) \cos \omega(t-x) d\omega dt$$

Using $\omega = u$ we have

$$f(x) = \frac{1}{\pi} \int_0^{\infty} \int_{-\infty}^{\infty} f(t) \cos u(t-x) du dt$$

$$f(x) = \frac{1}{\pi} \int_0^{\infty} \int_{-1}^1 \cos u(t-x) dt du \quad \text{since } f(t) = 1$$

Now integrating w.r.t. t we have

$$f(x) = \frac{1}{\pi} \int_0^\infty \left[\frac{\sin u(t-x)}{u} \right]_{-1}^1 du$$

$$f(x) = \frac{1}{\pi} \int_0^\infty \left[\frac{\sin u(1-x) + \sin u(1+x)}{u} \right] du$$

Now using $\sin C + \sin D = 2 \sin \frac{C+D}{2} \cos \frac{C-D}{2}$ and solving it we will get

$$f(x) = \frac{2}{\pi} \int_0^\infty \frac{\sin u \cos ux}{u} du$$

We can rewrite this

$$\int_0^\infty \frac{\sin u \cos ux}{u} du = \frac{\pi}{2} f(x)$$

$$\int_0^\infty \frac{\sin u \cos ux}{u} du = \begin{cases} \frac{\pi}{2} \times 1 = \frac{\pi}{2}, & \text{for } x < 1 \\ \frac{\pi}{2} \times 0 = 0, & \text{for } x > 1 \end{cases}$$

For $x=1$, which is a point of discontinuity of $f(x)$, value of integral = $\frac{\pi+0}{2} = \frac{\pi}{4}$

FOURIER TRANSFORMS

From the Fourier complex integral we know that

$$f(x) = \frac{1}{2\pi} \int_{-\infty}^\infty e^{-i\omega x} d\omega \int_{-\infty}^\infty f(t) e^{i\omega t} dt$$

We can rewrite the above expression as follows using $\omega = s$

$$f(x) = \frac{1}{2\pi} \int_{-\infty}^\infty e^{-isx} ds \int_{-\infty}^\infty f(t) e^{ist} dt = \left[\frac{1}{\sqrt{2\pi}} \int_{-\infty}^\infty e^{-isx} ds \right] \left[\frac{1}{\sqrt{2\pi}} \int_{-\infty}^\infty f(t) e^{ist} dt \right]$$

Now using $\frac{1}{\sqrt{2\pi}} \int_{-\infty}^{\infty} f(t) e^{ist} dt = F(s)$ in above equation, we get

$$f(x) = \frac{1}{\sqrt{2\pi}} \int_{-\infty}^{\infty} e^{-isx} F(s) ds$$

Where $F(s)$ is called the Fourier Transform of $f(x)$.

And $f(x)$ is called the Inverse Fourier transform of $F(s)$.

Thus , we obtain the definition of Fourier transform is

$$F(s) = F[f(x)] = \frac{1}{\sqrt{2\pi}} \int_{-\infty}^{\infty} f(t) e^{ist} dt$$

$$f(x) = \frac{1}{\sqrt{2\pi}} \int_{-\infty}^{\infty} e^{-isx} \cdot F(s) ds$$

FOURIER SINE TRANSFORMS

We know that from Fourier sine integral

$$f(x) = \frac{2}{\pi} \int_0^{\infty} \sin sx \, ds \int_0^{\infty} f(t) \sin st \, dt = \sqrt{\frac{2}{\pi}} \int_0^{\infty} \sin sx \, ds \left[\sqrt{\frac{2}{\pi}} \int_0^{\infty} f(t) \sin st \, dt \right]$$

$$\text{Now putting } F(s) = \sqrt{\frac{2}{\pi}} \int_0^{\infty} f(t) \sin st \, dt$$

We have

$$f(x) = \sqrt{\frac{2}{\pi}} \int_0^{\infty} \sin sx \, ds F(s)$$

In above equation $F(s)$ is called Fourier Sine transform of $f(x)$

$$\mathbf{F(s) = F_s [f(x)] = \sqrt{\frac{2}{\pi}} \int_0^{\infty} f(t) \sin st \, dt}$$

And $f(x)$ given below is known as inverse Fourier Sine transform of $F(s)$

$$\mathbf{f(x) = \sqrt{\frac{2}{\pi}} \int_0^{\infty} F(s) \sin sx \, ds}$$

FOURIER COSINE TRANSFORM

From Fourier cosine integral we know that

$$f(x) = \frac{2}{\pi} \int_0^{\infty} \cos \omega x \, d\omega \int_0^{\infty} f(t) \cos \omega t \, dt$$
$$f(x) = \sqrt{\frac{2}{\pi}} \int_0^{\infty} \cos sx \, ds \left[\sqrt{\frac{2}{\pi}} \int_0^{\infty} f(t) \cos st \, dt \right]$$

Now putting $F(s) = \sqrt{\frac{2}{\pi}} \int_0^{\infty} f(t) \cos st \, dt$

$$f(x) = \sqrt{\frac{2}{\pi}} \int_0^{\infty} \cos sx \, ds F(s)$$

In above equation $F(s)$ is called Fourier cosine transform of $f(x)$

$$\mathbf{F(s) = F_c [f(x)] = \sqrt{\frac{2}{\pi}} \int_0^{\infty} f(t) \cos st \, dt}$$

And $f(x)$ given below is known as inverse Fourier cosine transform of $F(s)$

$$\mathbf{f(x) = \sqrt{\frac{2}{\pi}} \int_0^{\infty} \cos sx \, F(s) \, ds}$$

Example 2: Find the Fourier transform of e^{-ax^2} , where $a > 0$.

Solution : The Fourier transform of $f(x)$:

$$F\{f(x)\} = \frac{1}{\sqrt{2\pi}} \int_{-\infty}^{\infty} f(x) e^{isx} dx$$

Hence

$$\begin{aligned} F\{e^{-ax^2}\} &= \frac{1}{\sqrt{2\pi}} \int_{-\infty}^{\infty} e^{-ax^2} e^{isx} dx = \frac{1}{\sqrt{2\pi}} \int_{-\infty}^{\infty} e^{-ax^2 + isx} dx \\ \Rightarrow F\{e^{-ax^2}\} &= \frac{1}{\sqrt{2\pi}} \int_{-\infty}^{\infty} e^{-ax^2 - \frac{s^2}{4a} + isx + \frac{s^2}{4a}} dx = \frac{1}{\sqrt{2\pi}} \int_{-\infty}^{\infty} e^{-\left(x\sqrt{a} - \frac{is}{2\sqrt{a}}\right)^2 - \frac{s^2}{4a}} dx \\ \Rightarrow F\{e^{-ax^2}\} &= \frac{e^{-\frac{s^2}{4a}}}{\sqrt{2\pi}} \int_{-\infty}^{\infty} e^{-\left(x\sqrt{a} - \frac{is}{2\sqrt{a}}\right)^2} dx \end{aligned}$$

Putting $x\sqrt{a} - \frac{is}{2\sqrt{a}} = u \Rightarrow dx = \frac{du}{\sqrt{a}}$ in above expression we get,

$$\begin{aligned} \Rightarrow F\{e^{-ax^2}\} &= \frac{e^{-\frac{s^2}{4a}}}{\sqrt{2\pi a}} \int_{-\infty}^{\infty} e^{-u^2} du \quad \left[\text{since } \int_{-\infty}^{\infty} e^{-x^2} dx = \sqrt{\pi} \right] \\ \Rightarrow F\{e^{-ax^2}\} &= \frac{e^{-\frac{s^2}{4a}}}{\sqrt{2\pi a}} \sqrt{\pi} = \frac{e^{-\frac{s^2}{4a}}}{\sqrt{2a}} \quad \text{Ans.} \end{aligned}$$

Example 3: Find the Fourier transform of

$$f(x) = \begin{cases} 2 & \text{for } |x| < a \\ 0 & \text{for } |x| > a \end{cases}$$

Solution: We know that the Fourier transform of a function is given by

$$F\{f(x)\} = \frac{1}{\sqrt{2\pi}} \int_{-\infty}^{\infty} f(x) e^{isx} dx$$

Using the given value of $f(x)$ we get,

$$\begin{aligned} F\{f(x)\} &= \frac{1}{\sqrt{2\pi}} \int_{-a}^a 2e^{isx} dx = \frac{2}{\sqrt{2\pi}} \int_{-a}^a e^{isx} dx = \\ F\{f(x)\} &= \frac{2}{\sqrt{2\pi}} \left[\frac{e^{isx}}{is} \right]_{-a}^a = \frac{2}{\sqrt{2\pi} is} [e^{ias} - e^{-ias}] = \frac{4}{\sqrt{2\pi} s} \frac{[e^{ias} - e^{-ias}]}{2i} \\ F\{f(x)\} &= \frac{4}{\sqrt{2\pi} s} \sin as = 2 \sqrt{\frac{2}{\pi}} \frac{\sin sa}{s} \quad \text{Ans.} \end{aligned}$$

Example 4: Find Fourier Sine transform of $\frac{1}{x}$.

Solution: We have to find the Fourier sine transform of $f(x) = \frac{1}{x}$

We know that from Fourier sine transform

$$F_s [f(x)] = \sqrt{\frac{2}{\pi}} \int_0^{\infty} f(x) \sin sx \, dx$$

Now using the value of $f(x) = \frac{1}{x}$, we get,

$$F_s [f(x)] = \sqrt{\frac{2}{\pi}} \int_0^{\infty} \frac{1}{x} \sin sx \, dx$$

$$\text{now using } sx = t \Rightarrow dx = \frac{dt}{s}$$

We get

$$= \sqrt{\frac{2}{\pi}} \int_0^{\infty} \frac{\sin t}{t} \, dt = \sqrt{\frac{2}{\pi}} \left(\frac{\pi}{2} \right) \Rightarrow \text{since } \int_0^{\infty} \frac{\sin t}{t} \, dt = \frac{\pi}{2}$$

Hence

$$F_s [f(x)] = \sqrt{\frac{\pi}{2}} \quad \text{Ans.}$$

Example 5: Find the Fourier Sine Transform of e^{-ax} .

Solution: Here, $f(x) = e^{-ax}$.

The Fourier sine transform of $f(x)$:

$$F_S [f(x)] = \sqrt{\frac{2}{\pi}} \int_0^{\infty} f(x) \sin sx \, dx$$

On putting the value of $f(x)$ in (1), we get

$$F_S [e^{-ax}] = \sqrt{\frac{2}{\pi}} \int_0^{\infty} e^{-ax} \sin sx \, dx$$

On Integrating by parts, we get

$$\begin{aligned} F_S [e^{-ax}] &= \sqrt{\frac{2}{\pi}} \left[\frac{e^{-ax}}{a^2 + s^2} [-a \sin sx - s \cos sx] \right]_0^{\infty} \\ \text{using } \left[\int_0^{\infty} e^{ax} \sin bx \, dx = \frac{e^{ax}}{a^2 + b^2} (a \sin bx - b \cos bx) \right] \\ &= \sqrt{\frac{2}{\pi}} \left[0 - \frac{1}{a^2 + s^2} (-s) \right] = \sqrt{\frac{2}{\pi}} \left(\frac{s}{a^2 + s^2} \right) \quad \text{Ans.} \end{aligned}$$

Example 6: Find the Fourier Cosine Transform of $f(x) = 5e^{-2x} + 2e^{-5x}$

Solution: The Fourier Cosine Transform of $f(x)$ is given by

$$F_c \{f(x)\} = \sqrt{\frac{2}{\pi}} \int_0^{\infty} f(x) \cos sx \, dx$$

Putting the value of $f(x)$, we get

$$\begin{aligned} F_c \{f(x)\} &= \sqrt{\frac{2}{\pi}} \int_0^{\infty} (5e^{-2x} + 2e^{-5x}) \cos sx \, dx \\ &= 5 \int_0^{\infty} e^{-2x} \cos sx \, dx + 2 \int_0^{\infty} e^{-5x} \cos sx \, dx \\ &\quad \text{using } \left[\int_0^{\infty} e^{ax} \cos bx \, dx = \frac{e^{ax}}{a^2 + b^2} (a \cos bx + b \sin bx) \right] \\ &= 5 \left[\frac{e^{-2x}}{(-2)^2 + s^2} (-2 \cos sx + s \sin sx) \right]_0^{\infty} + 2 \left[\frac{e^{-5x}}{(-5)^2 + s^2} (-5 \cos sx + s \sin sx) \right]_0^{\infty} \\ &= 5 \left[0 - \frac{1}{4 + s^2} (-2) \right] + 2 \left[0 - \frac{1}{25 + s^2} (-5) \right] = 5 \left(\frac{2}{s^2 + 4} \right) + 2 \left(\frac{5}{s^2 + 25} \right) \\ &= 10 \left(\frac{1}{s^2 + 4} + \frac{1}{s^2 + 25} \right) \quad \text{Ans.} \end{aligned}$$

PROPERTIES OF FOURIER TRANSFORMS

9.12.1 LINEAR PROPERTY: If $F_1(s)$ and $F_2(s)$ are Fourier transforms of $f_1(x)$ and $f_2(x)$ respectively then

$$F[af_1(x) + b f_2(x)] = a F_1(s) + b F_2(s) \quad \text{where } a \text{ and } b \text{ are constants.}$$

Proof: we know from the definition of Fourier transform

$$F(s) = \frac{1}{\sqrt{2\pi}} \int_{-\infty}^{\infty} f(x) e^{isx} dx$$

We can write

$$F_1(s) = \frac{1}{\sqrt{2\pi}} \int_{-\infty}^{\infty} f_1(x) e^{isx} dx$$

And

$$F_2(s) = \frac{1}{\sqrt{2\pi}} \int_{-\infty}^{\infty} f_2(x) e^{isx} dx$$

Now

$$\begin{aligned} F[af_1(x) + b f_2(x)] &= \frac{1}{\sqrt{2\pi}} \int_{-\infty}^{\infty} [af_1(x) + b f_2(x)] e^{isx} dx \\ &= a \frac{1}{\sqrt{2\pi}} \int_{-\infty}^{\infty} f_1(x) e^{isx} dx + b \frac{1}{\sqrt{2\pi}} \int_{-\infty}^{\infty} f_2(x) e^{isx} dx \\ \Rightarrow F[af_1(x) + b f_2(x)] &= a F_1(s) + b F_2(s) \quad \text{Proved} \end{aligned}$$

CHANGE OF SCALE PROPERTY

We know that Fourier transform equation is given by

$$F(s) = \frac{1}{\sqrt{2\pi}} \int_{-\infty}^{\infty} f(x) e^{isx} dx$$

Then

$$F\{f(ax)\} = \frac{1}{a} F\left(\frac{s}{a}\right)$$

Proof: we know

$$\begin{aligned} F(s) &= \frac{1}{\sqrt{2\pi}} \int_{-\infty}^{\infty} f(x) e^{isx} dx \\ \Rightarrow F\{f(ax)\} &= \frac{1}{\sqrt{2\pi}} \int_{-\infty}^{\infty} f(ax) e^{isx} dx \quad \left[\text{now put } ax = t \Rightarrow dx = \frac{dt}{a} \right] \end{aligned}$$

We have

$$\begin{aligned} F\{f(ax)\} &= \frac{1}{\sqrt{2\pi}} \int_{-\infty}^{\infty} f(t) e^{i\frac{s}{a}t} \frac{dt}{a} = \frac{1}{a} \frac{1}{\sqrt{2\pi}} \int_{-\infty}^{\infty} f(t) e^{i\left(\frac{s}{a}\right)t} dt \\ &\Rightarrow F\{f(ax)\} = \frac{1}{a} F\left(\frac{s}{a}\right) \quad \text{Proved} \end{aligned}$$

SHIFTING PROPERTY

The Fourier transform equation is given by

$$F(s) = \frac{1}{\sqrt{2\pi}} \int_{-\infty}^{\infty} f(x) e^{isx} dx$$

Then

$$F\{f(x - a)\} = e^{isa} F(s)$$

Proof: Given

$$F(s) = \frac{1}{\sqrt{2\pi}} \int_{-\infty}^{\infty} f(x) e^{isx} dx$$

then

$$F\{f(x - a)\} = \frac{1}{\sqrt{2\pi}} \int_{-\infty}^{\infty} f(x - a) e^{isx} dx$$

$$\text{Put } (x - a) = u \Rightarrow x = u + a \text{ and } dx = du$$

We have

$$F\{f(x - a)\} = \frac{1}{\sqrt{2\pi}} \int_{-\infty}^{\infty} f(u) e^{is(u+a)} du = e^{isa} \frac{1}{\sqrt{2\pi}} \int_{-\infty}^{\infty} f(u) e^{isu} du$$

$$\Rightarrow F\{f(x - a)\} = e^{isa} F(s) \quad \text{Proved}$$